boogieamp/src/boogie/controlflow/expression/CfgWildcardExpression.java
@@ -39,8 +39,8 @@ public class CfgWildcardExpression extends CfgExpression {
 	@Override
 	public String toString() {		
 		StringBuilder sb = new StringBuilder();
-		//TODO
-		return sb.toString();
+		throw new RuntimeException("wildcard not implemented");
+		//return sb.toString();
 	}
 
 	@Override
