boogieamp/src/boogie/expression/CodeExpression.java
@@ -1,0 +1,46 @@
+/**
+ * 
+ */
+package boogie.expression;
+
+import java.util.HashMap;
+
+import boogie.location.ILocation;
+import boogie.statement.Statement;
+
+/**
+ * @author schaef
+ *
+ */
+public class CodeExpression extends Expression {
+
+	Statement[] statements;
+	
+	public CodeExpression(ILocation loc, Statement[] stmts) {
+		super(loc);
+		this.statements = stmts;
+	}
+
+	public Statement[] getStatements() {
+		return this.statements;
+	}
+	
+	/**
+	 * Returns a textual description of this object.
+	 */
+	@Override
+	public String toString() {
+		return "CodeExpression";
+	}
+	
+	
+	/* (non-Javadoc)
+	 * @see boogie.expression.Expression#substitute(java.util.HashMap)
+	 */
+	@Override
+	public Expression substitute(HashMap<String, Expression> s) {
+		// TODO Auto-generated method stub
+		return null;
+	}
+
+}
