boogieamp_tests/src/boogieamp_tests/AllTests.java
@@ -1,0 +1,12 @@
+package boogieamp_tests;
+
+import org.junit.runner.RunWith;
+import org.junit.runners.Suite;
+import org.junit.runners.Suite.SuiteClasses;
+
+@RunWith(Suite.class)
+@SuiteClasses({ TestParse.class, TestParseOtherErrors.class,
+		TestParseParseErrors.class, TestParseTypeErrors.class })
+public class AllTests {
+
+}
